Prove wp_index__GetTuple

src/program_proof/mvcc/index_proof.v
@@ -4,17 +4,137 @@ From Perennial.program_proof Require Export disk_prelude.
 From Goose.github_com.mit_pdos.go_mvcc Require Import index.
 From Perennial.program_proof.mvcc Require Import mvcc_ghost tuple_proof.
 
+Local Ltac Zify.zify_post_hook ::= Z.div_mod_to_equations.
+
 Section heap.
 Context `{!heapGS Σ, !mvcc_ghostG Σ}.
 
-Definition is_index (idx : loc) (γ : mvcc_names) : iProp Σ := True.
+Definition own_index_bucket (bkt : loc) (γ : mvcc_names) : iProp Σ :=
+  ∃ (lockm : loc) (lockmM : gmap u64 loc),
+    "Hlockm" ∷ bkt ↦[IndexBucket :: "m"] #lockm ∗
+    "HlockmOwn" ∷ is_map lockm 1 lockmM ∗
+    "#HtuplesRP" ∷ ([∗ map] key ↦ tuple ∈ lockmM, is_tuple tuple key γ) ∗
+    "_" ∷ True.
+Local Hint Extern 1 (environments.envs_entails _ (own_index_bucket _ _)) => unfold own_index_bucket : core.
+  
+Definition is_index_bucket (bkt : loc) (γ : mvcc_names) : iProp Σ :=
+  ∃ (latch : loc) (lockm : loc)
+    (lockmM : gmap u64 loc),
+    "#Hlatch" ∷ readonly (bkt ↦[IndexBucket :: "latch"] #latch) ∗
+    "#HlatchRP" ∷ is_lock mvccN #latch (own_index_bucket bkt γ) ∗
+    "_" ∷ True.
 
+Definition N_IDX_BUCKET : nat := 2048.
+
+Definition is_index (idx : loc) (γ : mvcc_names) : iProp Σ :=
+  ∃ (bkts : Slice.t) (bktsL : list loc),
+    "#Hbkts" ∷ readonly (idx ↦[Index :: "buckets"] (to_val bkts)) ∗
+    (**
+     * Goose seems to translate accessing slices of structs (via [SliceGet] or [SlicePut])
+     * that have only one field to the type of that field, rather than the struct type.
+     * So here we use [ptrT] instead of [structTy Index].
+     *)
+    "#HbktsL" ∷ readonly (is_slice_small bkts ptrT 1 (to_val <$> bktsL)) ∗
+    "%HbktsLen" ∷ ⌜length bktsL = N_IDX_BUCKET⌝ ∗
+    "#HbktsRP" ∷ ([∗ list] _ ↦ bkt ∈ bktsL, is_index_bucket bkt γ) ∗ 
+    "_" ∷ True.
+
+(*****************************************************************)
+(* func (idx *Index) GetTuple(key uint64) *tuple.Tuple           *)
+(*****************************************************************)
 Theorem wp_index__GetTuple idx (key : u64) γ :
   is_index idx γ -∗
   {{{ True }}}
     Index__GetTuple #idx #key
   {{{ (tuple : loc), RET #tuple; is_tuple tuple key γ }}}.
 Proof.
-Admitted.
+  iIntros "#Hindex !>" (Φ) "_ HΦ".
+  iNamed "Hindex".
+  wp_call.
+
+  (***********************************************************)
+  (* b := getBucket(key)                                     *)
+  (* bucket := idx.buckets[b]                                *)
+  (***********************************************************)
+  wp_lam.
+  wp_pures.
+  wp_apply (wp_loadField_ro with "Hbkts").
+  iMod (readonly_load with "HbktsL") as (q) "HbktsL'".
+  list_elem bktsL (int.nat (word.modu key 2048)) as bkt.
+  { revert HbktsLen. rewrite /N_IDX_BUCKET. word. }
+  wp_apply (wp_SliceGet with "[$HbktsL']").
+  { iPureIntro.
+    rewrite list_lookup_fmap.
+    by rewrite Hbkt_lookup.
+  }
+  iIntros "[HbktsL' _]".
+  wp_pures.
+  (* Q: What's the relationship between [Absorbing] and [Persistent]? *)
+  iDestruct (big_sepL_lookup with "HbktsRP") as "HbktRP"; first done.
+  iNamed "HbktRP".
+
+  (***********************************************************)
+  (* bucket.latch.Lock()                                     *)
+  (* tupleCur, ok := bucket.m[key]                           *)
+  (***********************************************************)
+  wp_loadField.
+  wp_apply (acquire_spec with "HlatchRP").
+  iIntros "[Hlocked HbktOwn]".
+  iNamed "HbktOwn".
+  wp_pures.
+  wp_loadField.
+  wp_apply (wp_MapGet with "HlockmOwn").
+  iIntros (tuple ok) "[%Hmap_get HlockmOwn]".
+  wp_pures.
   
+  (***********************************************************)
+  (* if ok {                                                 *)
+  (*     bucket.latch.Unlock()                               *)
+  (*     return tupleCur                                     *)
+  (* }                                                       *)
+  (***********************************************************)
+  wp_if_destruct.
+  { (* The tuple is already in the index. *)
+    wp_loadField.
+    wp_apply (release_spec with "[-HΦ]").
+    { eauto 10 with iFrame. }
+    wp_pures.
+    iApply "HΦ".
+    iApply (big_sepM_lookup with "HtuplesRP").
+    by apply map_get_true.
+  }
+
+  (***********************************************************)
+  (* tupleNew := tuple.MkTuple()                             *)
+  (* bucket.m[key] = tupleNew                                *)
+  (* bucket.latch.Unlock()                                   *)
+  (***********************************************************)
+  apply map_get_false in Hmap_get as [Hlookup _].
+  clear tuple.
+  wp_apply wp_MkTuple.
+  iIntros (tuple) "#HtupleRP".
+  wp_pures.
+  wp_loadField.
+  wp_apply (wp_MapInsert with "HlockmOwn"); first done.
+  iIntros "HlockmOwn".
+  wp_pures.
+  wp_loadField.
+  wp_apply (release_spec with "[-HΦ HtupleRP]").
+  { iFrame "Hlocked HlatchRP".
+    iNext.
+    rewrite /own_index_bucket.
+    do 2 iExists _.
+    iFrame.
+    iSplit; last done.
+    iApply (big_sepM_insert with "[$HtuplesRP HtupleRP]"); first done.
+    iFrame "HtupleRP".
+  }
+  wp_pures.
+    
+  (***********************************************************)
+  (* return tupleNew                                         *)
+  (***********************************************************)
+  by iApply "HΦ".
+Qed.
+
 End heap.
